src/phl/ecPhlFun.mli
@@ -27,13 +27,19 @@ val subst_pre :
 (* -------------------------------------------------------------------- *)
 type p_upto_info = pformula * pformula * (pformula option)
 
-type abs_inv_inf = (xpath * form) list * (xpath * cost) list
+type abs_inv_inf = (EcPath.xpath * EcParsetree.ptybinding * EcFol.cost) list
 
 val process_p_abs_inv_inf :
   EcCoreGoal.tcenv1 ->
   EcEnv.LDecl.hyps ->
   p_abs_inv_inf ->
   abs_inv_inf
+
+val process_inv_pabs_inv_finfo:
+  EcCoreGoal.tcenv1 ->
+  pformula ->
+  p_abs_inv_inf ->
+  form * abs_inv_inf
 
 type inv_inf =  [
   | `Std     of cost
