theories/core/AllCore.ec
@@ -13,3 +13,28 @@ require export Core Int IntExtra Real RealExtra.
 schema cost_oget ['a] `{P} {o: 'a option} : 
   cost [P : oget o] = cost [P:o] + 1.
 hint simplify cost_oget.
+
+(* Cost on integer operations *)
+op cincr : int -> int.
+op ceqint : int -> int.
+op cltint : int -> int.
+op cleint : int -> int.
+
+axiom ge0_cincr m  : 0 <= cincr m.
+axiom ge0_ceqint m : 0 <= ceqint m.
+axiom ge0_cltint m : 0 <= cltint m.
+axiom ge0_cleint m : 0 <= cleint m.
+
+schema cost_incr {n:int} (m:int) : cost[`|n| <= m : n + 1] = cost[true:n] + cincr m.
+
+schema cost_eqint {n1 n2:int} (m:int) : 
+  cost[`|n1| <= m /\ `|n2| <= m : n1 = n2] = cost[true:n1] + cost[true:n2] + ceqint m.
+
+schema cost_ltint {n1 n2:int} (m:int) : 
+  cost[`|n1| <= m /\ `|n2| <= m : n1 < n2] = cost[true:n1] + cost[true:n2] + cltint m.
+
+schema cost_leint {n1 n2:int} (m:int) : 
+  cost[`|n1| <= m /\ `|n2| <= m : n1 < n2] = cost[true:n1] + cost[true:n2] + cleint m.
+
+
+hint simplify cost_incr, cost_eqint, cost_ltint, cost_leint.
