examples/hashed_elgamal_generic.ec
@@ -187,16 +187,14 @@ section.
     time [6 + cunifin + (3 + cunifin + cget qH + cset qH + cin qH) * (cA.`oguess + cA.`ochoose) + cA.`cguess + cA.`cchoose].
   proof.
     proc; wp.
-    call (_: bounded RO.m (size H.qs);
-           (H.o : size H.qs- cA.`ochoose) 
+    call (_: size H.qs- cA.`ochoose <= k /\ bounded RO.m (size H.qs);
            time
-           [(H.o : [fun _ => 3 + cunifin + cget qH + cset qH + cin qH])]).
+           [(H.o k : [3 + cunifin + cget qH + cset qH + cin qH])]).
     + move=> zo hzo; proc; inline *.
       wp := (bounded RO.m qH).
       by auto => &hr />; rewrite dbits_ll /=; smt (cset_pos bounded_set).
-    auto; call (_: bounded RO.m (size H.qs);
-           (H.o : size H.qs)
-           time [(H.o : [fun _ => 3 + cunifin + cget qH + cset qH + cin qH])]).
+    auto; call (_: size H.qs = k /\ bounded RO.m (size H.qs);
+           time [(H.o k : [3 + cunifin + cget qH + cset qH + cin qH])]).
     + move=> zo hzo; proc; inline *.
       wp := (bounded RO.m qH).
       auto => &hr />; rewrite dbits_ll /=; smt(cset_pos bounded_set cA_pos).
